Introduce ChaseDerivations with mem_rec principle

ExistentialRules/ChaseSequence/ChaseBranch.lean
@@ -6,202 +6,403 @@ import ExistentialRules.ChaseSequence.ChaseNode
 variable {sig : Signature} [DecidableEq sig.P] [DecidableEq sig.C] [DecidableEq sig.V]
 
 def exists_trigger_opt_fs (obs : ObsoletenessCondition sig) (rules : RuleSet sig) (before : ChaseNode obs rules) (after : Option (ChaseNode obs rules)) : Prop :=
-  ∃ trg : (RTrigger (obs : LaxObsoletenessCondition sig) rules), trg.val.active before.facts ∧ ∃ i, some {
-    facts := ⟨
-      before.facts ∪ (trg.val.mapped_head[i.val]'(i.isLt)).toSet,
-      by
-        rcases before.facts.property with ⟨l_before, _, l_eq⟩
-        let new_list := (l_before ++ trg.val.mapped_head[i.val]).eraseDupsKeepRight
-        exists new_list
-        constructor
-        . apply List.nodup_eraseDupsKeepRight
-        . intro e
-          unfold new_list
-          rw [List.mem_eraseDupsKeepRight, List.mem_append]
-          rw [l_eq]
-          simp only [Union.union, List.mem_toSet]
-          rfl
-    ⟩
+  ∃ trg : (RTrigger (obs : LaxObsoletenessCondition sig) rules), trg.val.active before.facts ∧ ∃ i, after = some {
+    facts := before.facts ∪ (trg.val.mapped_head[i.val]'(i.isLt)).toSet,
     origin := some ⟨trg, i⟩
     facts_contain_origin_result := by simp [Option.is_none_or]; apply Set.subset_union_of_subset_right; apply Set.subset_refl
-  } = after
+  }
 
 def not_exists_trigger_opt_fs (obs : ObsoletenessCondition sig) (rules : RuleSet sig) (before : ChaseNode obs rules) (after : Option (ChaseNode obs rules)) : Prop :=
   ¬(∃ trg : (RTrigger obs rules), trg.val.active before.facts) ∧ after = none
 
-structure ChaseBranch (obs : ObsoletenessCondition sig) (kb : KnowledgeBase sig) where
-  branch : PossiblyInfiniteList (ChaseNode obs kb.rules)
-  database_first : branch.head = some {
-    facts := (
-      let fs := kb.db.toFactSet
-      ⟨fs.val, fs.property.left⟩
-    ),
-    origin := none,
-    facts_contain_origin_result := by simp [Option.is_none_or]
-  }
+structure ChaseDerivation (obs : ObsoletenessCondition sig) (rules : RuleSet sig) where
+  branch : PossiblyInfiniteList (ChaseNode obs rules)
+  isSome_head : branch.head.isSome
   triggers_exist : ∀ n : Nat, (branch.drop n).head.is_none_or (fun before =>
     let after := (branch.drop n).tail.head
-    (exists_trigger_opt_fs obs kb.rules before after) ∨
-    (not_exists_trigger_opt_fs obs kb.rules before after))
-  fairness : ∀ trg : (RTrigger obs kb.rules), ∃ i : Nat, ((branch.drop i).head.is_some_and (fun fs => ¬ trg.val.active fs.facts))
+    (exists_trigger_opt_fs obs rules before after) ∨
+    (not_exists_trigger_opt_fs obs rules before after))
+  fairness : ∀ trg : (RTrigger obs rules), ∃ i : Nat, ((branch.drop i).head.is_some_and (fun fs => ¬ trg.val.active fs.facts))
     ∧ (∀ j : Nat, ((branch.drop i).tail.get? j).is_none_or (fun fs => ¬ trg.val.active fs.facts))
 
-namespace ChaseBranch
+namespace ChaseDerivation
 
-  variable {obs : ObsoletenessCondition sig} {kb : KnowledgeBase sig}
+  variable {obs : ObsoletenessCondition sig} {rules : RuleSet sig}
 
-  def result (cb : ChaseBranch obs kb) : FactSet sig :=
-    fun f => ∃ n : Nat, (cb.branch.get? n).is_some_and (fun fs => f ∈ fs.facts.val)
+  instance : Membership (ChaseNode obs rules) (ChaseDerivation obs rules) where
+    mem cd node := node ∈ cd.branch
 
-  theorem predecessor_isSome_of_isSome (cb : ChaseBranch obs kb) (i : Nat) (isSome : (cb.branch.drop i).tail.head.isSome) :
-      (cb.branch.drop i).head.isSome := by
-    cases eq : (cb.branch.drop i).head with
-    | none =>
-      have : (cb.branch.drop i).tail.head = none := by apply cb.branch.no_holes; exact eq
-      simp [this] at isSome
-    | some _ => simp
+  def result (cd : ChaseDerivation obs rules) : FactSet sig :=
+    fun f => ∃ node ∈ cd, f ∈ node.facts
 
-  def prev_node (cb : ChaseBranch obs kb) (i : Nat) (isSome : (cb.branch.drop i).tail.head.isSome) : ChaseNode obs kb.rules :=
-    (cb.branch.drop i).head.get (cb.predecessor_isSome_of_isSome i isSome)
+  -- inspired by List.IsSuffix; see https://github.com/leanprover/lean4/blob/9d4ad1273f6cea397c3066c2c83062a4410d16bf/src/Init/Data/List/Basic.lean#L1205
+  def IsSuffix (cd1 cd2 : ChaseDerivation obs rules) : Prop := cd1.branch <:+ cd2.branch
+  infixl:50 " <:+ " => IsSuffix
 
-  theorem prev_node_eq (cb : ChaseBranch obs kb) (i : Nat) (isSome : (cb.branch.drop i).tail.head.isSome) :
-      (cb.branch.drop i).head = some (cb.prev_node i isSome) := by
-    simp [prev_node]
+  theorem mem_of_mem_suffix {cd1 cd2 : ChaseDerivation obs rules} (suffix : cd1 <:+ cd2) : ∀ node ∈ cd1, node ∈ cd2 := by
+    rintro node ⟨n, node_eq⟩
+    rcases suffix with ⟨m, suffix⟩
+    exists m + n
+    rw [← suffix, InfiniteList.get_drop] at node_eq
+    exact node_eq
 
-  theorem origin_isSome (cb : ChaseBranch obs kb) (i : Nat) {node : ChaseNode obs kb.rules}
-      (eq : (cb.branch.drop i).tail.head = some node) : node.origin.isSome := by
-    have trg_ex := cb.triggers_exist i
-    rw [prev_node_eq _ _ (by simp [eq]), Option.is_none_or] at trg_ex
+  def derivation_for_branch_suffix
+      (cd : ChaseDerivation obs rules)
+      (l2 : PossiblyInfiniteList (ChaseNode obs rules))
+      (suffix : l2 <:+ cd.branch)
+      (l2_head_some : l2.head.isSome) :
+      ChaseDerivation obs rules where
+    branch := l2
+    isSome_head := l2_head_some
+    triggers_exist := by
+      rw [PossiblyInfiniteList.IsSuffix_iff] at suffix
+      rcases suffix with ⟨m, suffix⟩
+      rw [← suffix]
+      intro n
+      have := cd.triggers_exist (m + n)
+      simp only [PossiblyInfiniteList.head_drop, PossiblyInfiniteList.get?_drop] at *
+      exact this
+    fairness := by
+      rw [Option.isSome_iff_exists] at l2_head_some; rcases l2_head_some with ⟨l2_head, l2_head_eq⟩
+      rw [PossiblyInfiniteList.IsSuffix_iff] at suffix
+      rcases suffix with ⟨m, suffix⟩
+      rw [← suffix]
+      intro trg
+      rcases cd.fairness trg with ⟨i, fairness⟩
+      cases Decidable.em (i < m) with
+      | inl lt =>
+        rcases Nat.exists_eq_add_of_lt lt with ⟨diff, lt⟩
+        exists 0
+        constructor
+        . have fairness := fairness.right diff
+          rw [Option.is_none_or_iff] at fairness
+          rw [Option.is_some_and_iff]
+          simp only [PossiblyInfiniteList.drop_zero]
+          exists l2_head; constructor
+          . rw [suffix, l2_head_eq]
+          . apply fairness
+            rw [PossiblyInfiniteList.get?_tail, PossiblyInfiniteList.get?_drop, ← PossiblyInfiniteList.head_drop, Nat.succ_eq_add_one, ← Nat.add_assoc, ← lt]
+            rw [suffix, l2_head_eq]
+        . intro j
+          have fairness := fairness.right (diff.succ + j)
+          simp only [PossiblyInfiniteList.drop_zero, PossiblyInfiniteList.get?_tail, PossiblyInfiniteList.get?_drop] at *
+          have : (i + diff + 1 + j.succ) = (i + (diff.succ + j).succ) := by omega
+          rw [lt, this]
+          exact fairness
+      | inr le =>
+        have le := Nat.le_of_not_lt le
+        simp only [PossiblyInfiniteList.tail_drop, PossiblyInfiniteList.head_drop, PossiblyInfiniteList.get?_drop, Nat.succ_add] at *
+        exists (i - m)
+        simp only [← Nat.add_succ, ← Nat.add_assoc, Nat.add_sub_of_le le] at *
+        exact fairness
+
+  theorem fairness' {cd : ChaseDerivation obs rules} : ∀ (trg : RTrigger obs rules), ∃ (cd2 : ChaseDerivation obs rules), cd2 <:+ cd ∧ ∀ node ∈ cd2, ¬ trg.val.active node.facts := by
+    intro trg
+    rcases cd.fairness trg with ⟨n, fairness_head, fairness_tail⟩
+    rw [Option.is_some_and_iff] at fairness_head
+    rcases fairness_head with ⟨node, node_eq, fairness_head⟩
+    exists cd.derivation_for_branch_suffix (cd.branch.drop n) (cd.branch.IsSuffix_drop n) (by simp [node_eq])
+    constructor
+    . exact cd.branch.IsSuffix_drop n
+    . intro node2 node2_mem
+      rcases node2_mem with ⟨m, node2_mem⟩
+      simp only [derivation_for_branch_suffix, PossiblyInfiniteList.drop, InfiniteList.get_drop] at node2_mem
+      cases m with
+      | zero => simp only [PossiblyInfiniteList.head_drop, PossiblyInfiniteList.get?] at node_eq; rw [Nat.add_zero, node_eq, Option.some_inj] at node2_mem; rw [← node2_mem]; exact fairness_head
+      | succ m =>
+        specialize fairness_tail m
+        simp only [PossiblyInfiniteList.get?_tail, PossiblyInfiniteList.get?_drop] at fairness_tail
+        simp only [PossiblyInfiniteList.get?] at fairness_tail
+        simp only [node2_mem, Option.is_none_or] at fairness_tail
+        exact fairness_tail
+
+  def head (cd : ChaseDerivation obs rules) : ChaseNode obs rules := cd.branch.head.get (cd.isSome_head)
+  theorem head_mem {cd : ChaseDerivation obs rules} : cd.head ∈ cd := by exists 0; simp [head, PossiblyInfiniteList.head_eq, PossiblyInfiniteList.get?]
+
+  theorem subderivation_of_node_mem {cd : ChaseDerivation obs rules} {node : ChaseNode obs rules} (node_mem : node ∈ cd) :
+      ∃ (cd2 : ChaseDerivation obs rules), cd2.head = node ∧ cd2 <:+ cd := by
+    rcases node_mem with ⟨n, node_mem⟩
+    exists cd.derivation_for_branch_suffix (cd.branch.drop n) (cd.branch.IsSuffix_drop n) (by simp only [PossiblyInfiniteList.head_drop, PossiblyInfiniteList.get?, node_mem]; simp)
+    constructor
+    . simp only [derivation_for_branch_suffix, head, PossiblyInfiniteList.head_drop, PossiblyInfiniteList.get?, node_mem, Option.get_some]
+    . exact cd.branch.IsSuffix_drop n
+
+  def Node (cd : ChaseDerivation obs rules) := { node : ChaseNode obs rules // node ∈ cd}
+
+  def Node.cast_suffix {cd cd2 : ChaseDerivation obs rules} (suffix : cd <:+ cd2) (node : Node cd) : Node cd2 := ⟨node.val, mem_of_mem_suffix suffix _ node.property⟩
+
+  def predecessor {cd : ChaseDerivation obs rules} (n1 n2 : Node cd) : Prop := ∃ cd2, cd2 <:+ cd ∧ cd2.head = n1.val ∧ n2.val ∈ cd2
+  infixl:50 " ≼ " => predecessor
+
+  theorem predecessor_refl {cd : ChaseDerivation obs rules} {node : Node cd} : node ≼ node := by rcases cd.subderivation_of_node_mem node.property with ⟨cd2, head_eq, suffix⟩; exists cd2; simp only [suffix, head_eq, true_and]; rw [← head_eq]; exact cd2.head_mem
+  theorem predecessor_of_suffix {cd cd2 : ChaseDerivation obs rules} {n1 n2 : Node cd} (suffix : cd <:+ cd2) : n1 ≼ n2 -> (n1.cast_suffix suffix) ≼ (n2.cast_suffix suffix) := by
+    rintro ⟨cd3, suffix', head_eq, mem⟩
+    exists cd3; constructor
+    . exact cd3.branch.IsSuffix_trans suffix' suffix
+    constructor
+    . rw [head_eq]; rfl
+    . exact mem
+
+  def next (cd : ChaseDerivation obs rules) : Option (ChaseNode obs rules) := cd.branch.tail.head
+  theorem next_mem_of_mem {cd : ChaseDerivation obs rules} : ∀ next ∈ cd.next, next ∈ cd := by intro next next_mem; apply cd.branch.tail.mem_of_mem_suffix cd.branch.IsSuffix_tail; apply cd.branch.tail.head_mem; exact next_mem
+  theorem isSome_origin_next {cd : ChaseDerivation obs rules} {next : ChaseNode obs rules} (eq : cd.next = some next) : next.origin.isSome := by
+    have trg_ex := cd.triggers_exist 0
+    rw [PossiblyInfiniteList.drop_zero, Option.is_none_or_iff] at trg_ex
+    specialize trg_ex cd.head (by simp [head])
     cases trg_ex with
-    | inl trg_ex =>
-      unfold exists_trigger_opt_fs at trg_ex
-      rcases trg_ex with ⟨trg, _, disj, trg_eq⟩
-      simp only [eq] at trg_eq
-      injection trg_eq with trg_eq
-      rw [← trg_eq]
-      simp
-    | inr trg_ex =>
-      unfold not_exists_trigger_opt_fs at trg_ex
-      simp only [eq] at trg_ex
-      simp at trg_ex
-
-  theorem origin_trg_is_active (cb : ChaseBranch obs kb) (i : Nat) (node : ChaseNode obs kb.rules) (eq : (cb.branch.drop i).tail.head = some node) :
-      (node.origin.get (cb.origin_isSome i eq)).fst.val.active (cb.prev_node i (by simp [eq])).facts.val := by
-    have trg_ex := cb.triggers_exist i
-    rw [prev_node_eq _ _ (by simp [eq]), Option.is_none_or] at trg_ex
+    | inl trg_ex => rcases trg_ex with ⟨_, _, _, trg_ex⟩; unfold ChaseDerivation.next at eq; rw [eq, Option.some_inj] at trg_ex; rw [trg_ex]; simp
+    | inr trg_ex => have contra := trg_ex.right; unfold ChaseDerivation.next at eq; simp [eq] at contra
+  theorem active_trigger_origin_next {cd : ChaseDerivation obs rules} {next : ChaseNode obs rules} (eq : cd.next = some next) :
+      (next.origin.get (cd.isSome_origin_next eq)).fst.val.active cd.head.facts := by
+    have trg_ex := cd.triggers_exist 0
+    rw [PossiblyInfiniteList.drop_zero, Option.is_none_or_iff] at trg_ex
+    specialize trg_ex cd.head (by simp [head])
     cases trg_ex with
-    | inr trg_ex => unfold not_exists_trigger_opt_fs at trg_ex; rw [trg_ex.right] at eq; simp at eq
-    | inl trg_ex =>
-      unfold exists_trigger_opt_fs at trg_ex
-      rcases trg_ex with ⟨trg, trg_active, disj, trg_eq⟩
-      simp only [eq] at trg_eq
-      injection trg_eq with trg_eq
-      simp only [← trg_eq]
-      exact trg_active
-
-  theorem origin_trg_result_yields_next_node_facts (cb : ChaseBranch obs kb) (i : Nat) (node : ChaseNode obs kb.rules) (eq : (cb.branch.drop i).tail.head = some node) :
-      node.facts.val = (cb.prev_node i (by simp [eq])).facts.val ∪ (node.origin_result (cb.origin_isSome i eq)).toSet := by
-    have trg_ex := cb.triggers_exist i
-    rw [prev_node_eq _ _ (by simp [eq]), Option.is_none_or] at trg_ex
+    | inl trg_ex => rcases trg_ex with ⟨trg', trg'_active, _, trg_ex⟩; unfold ChaseDerivation.next at eq; rw [eq, Option.some_inj] at trg_ex; simp only [trg_ex, Option.get_some]; exact trg'_active
+    | inr trg_ex => have contra := trg_ex.right; unfold ChaseDerivation.next at eq; simp [eq] at contra
+  theorem isSome_next_iff_trg_ex {cd : ChaseDerivation obs rules} : cd.next.isSome ↔ ∃ (trg : RTrigger obs rules), trg.val.active cd.head.facts := by
+    constructor
+    . rw [Option.isSome_iff_exists]
+      rintro ⟨next, eq⟩
+      exists (next.origin.get (cd.isSome_origin_next eq)).fst
+      exact active_trigger_origin_next eq
+    . rintro ⟨trg, active⟩
+      apply Decidable.byContradiction
+      rw [Option.not_isSome_iff_eq_none]
+      intro eq_none
+      have trg_ex := cd.triggers_exist 0
+      rw [PossiblyInfiniteList.drop_zero, Option.is_none_or_iff] at trg_ex
+      specialize trg_ex cd.head (by simp [head])
+      cases trg_ex with
+      | inl trg_ex => rcases trg_ex with ⟨_, _, _, contra⟩; unfold next at eq_none; simp [eq_none] at contra
+      | inr trg_ex => apply trg_ex.left; exists trg
+  theorem facts_next {cd : ChaseDerivation obs rules} {next : ChaseNode obs rules} (eq : cd.next = some next) :
+      next.facts = cd.head.facts ∪ (next.origin_result (cd.isSome_origin_next eq)).toSet := by
+    have trg_ex := cd.triggers_exist 0
+    rw [PossiblyInfiniteList.drop_zero, Option.is_none_or_iff] at trg_ex
+    specialize trg_ex cd.head (by simp [head])
     cases trg_ex with
-    | inr trg_ex => unfold not_exists_trigger_opt_fs at trg_ex; rw [trg_ex.right] at eq; simp at eq
-    | inl trg_ex =>
-      unfold exists_trigger_opt_fs at trg_ex
-      rcases trg_ex with ⟨trg, trg_active, disj, trg_eq⟩
-      simp only [eq] at trg_eq
-      injection trg_eq with trg_eq
-      simp only [← trg_eq]
-      unfold ChaseNode.origin_result
-      simp
+    | inl trg_ex => rcases trg_ex with ⟨trg', trg'_active, _, trg_ex⟩; unfold ChaseDerivation.next at eq; rw [eq, Option.some_inj] at trg_ex; simp only [trg_ex]; rfl
+    | inr trg_ex => have contra := trg_ex.right; unfold ChaseDerivation.next at eq; simp [eq] at contra
 
-  theorem stepIsSubsetOfAllFollowing (cb : ChaseBranch obs kb) (i : Nat) (node : ChaseNode obs kb.rules) (eq : (cb.branch.drop i).head = some node) :
-      ∀ j, ((cb.branch.drop i).get? j).is_none_or (fun node2 => node.facts.val ⊆ node2.facts.val) := by
-    intro j
-    induction j with
-    | zero => rw [← PossiblyInfiniteList.head_eq, eq]; simp only [Option.is_none_or]; apply Set.subset_refl
-    | succ j ih =>
-      rw [Option.is_none_or_iff]
-      intro node2 eq2
-      let prev_node := (cb.prev_node (i + j) (by rw [PossiblyInfiniteList.head_eq, PossiblyInfiniteList.get?_tail, PossiblyInfiniteList.get?_drop]; rw [PossiblyInfiniteList.get?_drop, ← Nat.add_assoc] at eq2; rw [eq2]; simp))
-      apply Set.subset_trans (b := prev_node.facts.val)
-      . rw [Option.is_none_or_iff] at ih
-        specialize ih prev_node (by apply cb.prev_node_eq)
+  theorem head_prec_next {cd : ChaseDerivation obs rules} : ∀ {next}, (mem : next ∈ cd.next) -> ⟨cd.head, cd.head_mem⟩ ≼ ⟨next, cd.next_mem_of_mem _ mem⟩ := by
+    intro next next_mem; exact ⟨cd, cd.branch.IsSuffix_refl, rfl, cd.next_mem_of_mem _ next_mem⟩
+
+  theorem mem_rec
+      {cd : ChaseDerivation obs rules}
+      {motive : Node cd -> Prop}
+      (head : motive ⟨cd.head, cd.head_mem⟩)
+      (step : ∀ (cd2 : ChaseDerivation obs rules), (suffix : cd2 <:+ cd) -> motive ⟨cd2.head, mem_of_mem_suffix suffix _ cd2.head_mem⟩ -> ∀ next, (next_mem : next ∈ cd2.next) -> motive ⟨next, mem_of_mem_suffix suffix _ (cd2.next_mem_of_mem _ next_mem)⟩)
+      (node : Node cd) :
+      motive node := by
+    induction node using PossiblyInfiniteList.mem_rec with
+    | head head' mem => unfold ChaseDerivation.head at head; rw [Option.mem_def] at mem; simp only [mem, Option.get_some] at head; exact head
+    | step l2 suffix ih next next_mem =>
+      rcases ih with ⟨head, head_mem, ih⟩
+      let cd2 : ChaseDerivation obs rules := cd.derivation_for_branch_suffix l2 suffix (by rw [head_mem]; simp)
+      apply step cd2 suffix
+      . simp only [cd2, derivation_for_branch_suffix, ChaseDerivation.head];
+        conv => right; left; left; rw [head_mem]
+        simp only [Option.get_some]
         exact ih
-      . rw [cb.origin_trg_result_yields_next_node_facts (i + j) node2 eq2]
-        apply Set.subset_union_of_subset_left
-        apply Set.subset_refl
+      . exact next_mem
 
-  theorem stepIsSubsetOfResult (cb : ChaseBranch obs kb) : ∀ n : Nat, (cb.branch.get? n).is_none_or (fun fs => fs.facts.val ⊆ cb.result) := by
-    intro n
-    rw [Option.is_none_or_iff]
-    intro fs _
-    intro f h
-    exists n
-    rw [Option.is_some_and_iff]
-    exists fs
+  def tail (cd : ChaseDerivation obs rules) (next_some : cd.next.isSome) : ChaseDerivation obs rules :=
+    cd.derivation_for_branch_suffix cd.branch.tail (cd.branch.IsSuffix_tail) next_some
+  theorem head_tail {cd : ChaseDerivation obs rules} {next_some : cd.next.isSome} : some (cd.tail next_some).head = cd.next := by
+    unfold tail head ChaseDerivation.next derivation_for_branch_suffix
+    simp only [Option.some_get]
+  theorem head_tail' {cd : ChaseDerivation obs rules} {next_some : cd.next.isSome} : (cd.tail next_some).head = cd.next.get next_some := by rfl
 
-  theorem constantsInStepAreFromDatabaseOrRuleSet (cb : ChaseBranch obs kb) (i : Nat) (node : ChaseNode obs kb.rules) (eq : cb.branch.get? i = some node) :
-      node.facts.val.constants ⊆ (kb.db.constants.val ∪ kb.rules.head_constants) := by
-    induction i generalizing node with
-    | zero =>
-      rw [← PossiblyInfiniteList.head_eq, cb.database_first] at eq
-      injection eq with eq
-      rw [← eq]
-      rw [Database.toFactSet_constants_same]
+  theorem suffix_iff_eq_or_suffix_tail {cd1 cd2 : ChaseDerivation obs rules} : cd1 <:+ cd2 ↔ cd1 = cd2 ∨ ∃ h, cd1 <:+ cd2.tail h := by
+    -- TODO: maybe we should extract a result like this to InfiniteList directly
+    constructor
+    . rintro ⟨n, suffix⟩
+      cases n with
+      | zero => apply Or.inl; rw [InfiniteList.drop_zero] at suffix; apply Eq.symm; rw [ChaseDerivation.mk.injEq, PossiblyInfiniteList.mk.injEq]; exact suffix
+      | succ n =>
+        apply Or.inr
+        exists (by
+          rw [Option.isSome_iff_ne_none]
+          intro contra
+          have := cd2.branch.get?_eq_none_of_le_of_eq_none contra (n+1) (by simp)
+          simp only [PossiblyInfiniteList.get?] at this
+          rw [InfiniteList.ext_iff] at suffix
+          specialize suffix 0
+          rw [InfiniteList.get_drop, Nat.add_zero, this] at suffix
+          have contra := cd1.isSome_head
+          rw [Option.isSome_iff_ne_none] at contra
+          apply contra
+          simp only [PossiblyInfiniteList.head_eq, PossiblyInfiniteList.get?]
+          rw [← suffix])
+        exists n
+        simp only [tail, derivation_for_branch_suffix, PossiblyInfiniteList.tail]
+        apply InfiniteList.ext
+        intro m
+        simp only [InfiniteList.get_tail, InfiniteList.get_drop]
+        rw [InfiniteList.ext_iff] at suffix
+        simp only [InfiniteList.get_drop] at suffix
+        have : (n+m).succ = (n + 1 + m) := by omega
+        rw [this]
+        apply suffix m
+    . intro h; cases h with
+      | inl eq => rw [eq]; exact PossiblyInfiniteList.IsSuffix_refl
+      | inr suffix => rcases suffix with ⟨h, suffix⟩; apply PossiblyInfiniteList.IsSuffix_trans suffix; exact PossiblyInfiniteList.IsSuffix_tail
+
+  theorem mem_tail_iff {cd : ChaseDerivation obs rules} {next_some : cd.next.isSome} {node : ChaseNode obs rules} :
+      node ∈ cd.tail next_some ↔ ∃ cd2, cd2 <:+ cd ∧ cd2.next = some node := by
+    constructor
+    . intro node_mem
+      let node' : (cd.tail next_some).Node := ⟨node, node_mem⟩
+      show ∃ cd2, cd2 <:+ cd ∧ cd2.next = some node'.val
+      induction node' using mem_rec with
+      | head => exists cd; constructor; exact cd.branch.IsSuffix_refl; rw [head_tail]
+      | step cd3 suffix ih next next_mem =>
+        exists cd3; constructor
+        . apply cd3.branch.IsSuffix_trans suffix; exact cd.branch.IsSuffix_tail
+        . exact next_mem
+    . rintro ⟨cd2, suffix, next_eq⟩
+      have : cd2.tail (by simp [next_eq]) <:+ cd.tail next_some := by
+        -- TODO: maybe we should extract a result like this to InfiniteList directly
+        rcases suffix with ⟨n, suffix⟩
+        exists n
+        simp only [tail, derivation_for_branch_suffix, PossiblyInfiniteList.tail]
+        apply InfiniteList.ext
+        intro m
+        simp only [InfiniteList.get_tail, InfiniteList.get_drop]
+        rw [InfiniteList.ext_iff] at suffix
+        simp only [InfiniteList.get_drop] at suffix
+        apply suffix m.succ
+      apply mem_of_mem_suffix this
+      rw [← head_tail (next_some := by simp [next_eq]), Option.some_inj] at next_eq
+      simp only [← next_eq]
+      apply head_mem
+
+  theorem facts_node_subset_every_mem {cd : ChaseDerivation obs rules} : ∀ node ∈ cd, cd.head.facts ⊆ node.facts := by
+    intro node node_mem
+    let node' : cd.Node := ⟨node, node_mem⟩
+    show cd.head.facts ⊆ node'.val.facts
+    induction node' using mem_rec with
+    | head => apply Set.subset_refl
+    | step cd2 suffix subset next next_eq =>
+      apply Set.subset_trans subset
+      rw [cd2.facts_next next_eq]
       apply Set.subset_union_of_subset_left
       apply Set.subset_refl
-    | succ i ih =>
-      let prev_node := (cb.prev_node i (by simp [PossiblyInfiniteList.head_eq, PossiblyInfiniteList.get?_tail, PossiblyInfiniteList.get?_drop, eq]))
 
-      rw [cb.origin_trg_result_yields_next_node_facts i node eq]
-      unfold FactSet.constants
+  theorem facts_node_subset_of_prec {cd : ChaseDerivation obs rules} {node1 node2 : cd.Node} : node1 ≼ node2 -> node1.val.facts ⊆ node2.val.facts := by
+    rintro ⟨cd2, suffix, head_eq, mem⟩
+    rw [← head_eq]
+    apply facts_node_subset_every_mem
+    exact mem
+
+  theorem facts_node_subset_result {cd : ChaseDerivation obs rules} : ∀ node ∈ cd, node.facts ⊆ cd.result := by intro node _ _ _; exists node
+
+  theorem head_not_mem_tail {cd : ChaseDerivation obs rules} : ∀ h, ¬ cd.head ∈ cd.tail h := by
+    intro h contra
+    rw [mem_tail_iff] at contra
+    rcases contra with ⟨cd2, suffix, contra⟩
+    apply (cd2.active_trigger_origin_next contra).right
+    apply obs.contains_trg_result_implies_cond
+    have := cd.head.facts_contain_origin_result
+    rw [Option.is_none_or_iff] at this
+    specialize this (cd.head.origin.get (cd2.isSome_origin_next contra)) (by simp)
+    apply Set.subset_trans this
+    apply cd.facts_node_subset_every_mem
+    apply mem_of_mem_suffix suffix
+    exact cd2.head_mem
+
+  theorem eq_of_suffix_of_head_mem {cd1 cd2 : ChaseDerivation obs rules} (suffix : cd1 <:+ cd2) (head_mem : cd2.head ∈ cd1) : cd1 = cd2 := by
+    rw [suffix_iff_eq_or_suffix_tail] at suffix
+    cases suffix with
+    | inl suffix => exact suffix
+    | inr suffix => rcases suffix with ⟨h, suffix⟩; apply False.elim; apply head_not_mem_tail h; apply mem_of_mem_suffix suffix; exact head_mem
+
+  theorem predecessor_trans {cd : ChaseDerivation obs rules} {n1 n2 n3 : Node cd} : n1 ≼ n2 -> n2 ≼ n3 -> n1 ≼ n3 := by
+    rintro ⟨cd1, suffix1, head_eq1, prec1⟩ ⟨cd2, suffix2, head_eq2, prec2⟩
+    exists cd1; simp only [suffix1, head_eq1, true_and]
+    apply mem_of_mem_suffix _ _ prec2
+    cases PossiblyInfiniteList.suffix_or_suffix_of_suffix suffix1 suffix2 with
+    | inr suffix => exact suffix
+    | inl suffix => rw [eq_of_suffix_of_head_mem suffix]; exact PossiblyInfiniteList.IsSuffix_refl; rw [head_eq2]; exact prec1
+
+  theorem predecessor_antisymm {cd : ChaseDerivation obs rules} {n1 n2 : Node cd} : n1 ≼ n2 -> n2 ≼ n1 -> n1 = n2 := by
+    rintro ⟨cd1, suffix1, head_eq1, prec1⟩ ⟨cd2, suffix2, head_eq2, prec2⟩
+    have : cd1 = cd2 := by
+      cases PossiblyInfiniteList.suffix_or_suffix_of_suffix suffix1 suffix2 with
+      | inl suffix => rw [eq_of_suffix_of_head_mem suffix]; rw [head_eq2]; exact prec1
+      | inr suffix => rw [eq_of_suffix_of_head_mem suffix]; rw [head_eq1]; exact prec2
+    apply Subtype.ext
+    rw [← head_eq1, ← head_eq2, this]
+
+  theorem mem_suffix_of_mem {cd1 cd2 : ChaseDerivation obs rules} (suffix : cd1 <:+ cd2) : ∀ node ∈ cd2, node.facts ⊆ cd1.head.facts ∨ node ∈ cd1 := by
+    intro node node_mem
+    rcases subderivation_of_node_mem node_mem with ⟨cd3, cd3_head, suffix'⟩
+    cases PossiblyInfiniteList.suffix_or_suffix_of_suffix suffix suffix' with
+    | inl suffix => apply Or.inl; rw [← cd3_head]; apply cd3.facts_node_subset_every_mem; apply mem_of_mem_suffix suffix; apply cd1.head_mem
+    | inr suffix => apply Or.inr; rw [← cd3_head]; apply mem_of_mem_suffix suffix; apply cd3.head_mem
+
+  theorem result_suffix {cd1 cd2 : ChaseDerivation obs rules} (suffix : cd1 <:+ cd2) : cd1.result = cd2.result := by
+    apply Set.ext
+    intro f
+    constructor
+    . rintro ⟨node, node_mem, f_mem⟩; apply cd2.facts_node_subset_result; exact mem_of_mem_suffix suffix _ node_mem; exact f_mem
+    . rintro ⟨node, node_mem, f_mem⟩
+      cases mem_suffix_of_mem suffix _ node_mem with
+      | inl mem_suffix => apply cd1.facts_node_subset_result; exact cd1.head_mem; apply mem_suffix; exact f_mem
+      | inr mem_suffix => apply cd1.facts_node_subset_result; exact mem_suffix; exact f_mem
+
+  theorem constants_node_subset_constants_fs_union_constants_rules {cd : ChaseDerivation obs rules} {node : ChaseNode obs rules} (node_mem : node ∈ cd) :
+      node.facts.constants ⊆ (cd.head.facts.constants ∪ rules.head_constants) := by
+    let node' : cd.Node := ⟨node, node_mem⟩
+    show node'.val.facts.constants ⊆ (cd.head.facts.constants ∪ rules.head_constants)
+    induction node' using mem_rec with
+    | head =>
+      apply Set.subset_union_of_subset_left
+      apply Set.subset_refl
+    | step cd2 suffix ih next next_eq =>
+      rw [facts_next next_eq]
       intro c c_mem
-      rcases c_mem with ⟨f, f_mem, c_mem⟩
-      cases f_mem with
-      | inl f_mem =>
-        apply ih prev_node
-        . apply cb.prev_node_eq
-        . exists f
-      | inr f_mem =>
-        unfold ChaseNode.origin_result at f_mem
-        let origin := node.origin.get (cb.origin_isSome i eq)
-        have c_mem : c ∈ FactSet.constants (origin.fst.val.mapped_head[origin.snd.val]).toSet := by unfold FactSet.constants; exists f
+      rw [FactSet.constants_union] at c_mem
+      cases c_mem with
+      | inl c_mem => apply ih; exact c_mem
+      | inr c_mem =>
+        let origin := next.origin.get (cd2.isSome_origin_next next_eq)
         apply Set.subset_trans (origin.fst.val.mapped_head_constants_subset origin.snd)
         . intro c c_mem
           rw [List.mem_toSet, List.mem_append] at c_mem
           cases c_mem with
           | inl c_mem =>
-            apply ih prev_node
-            . apply cb.prev_node_eq
-            . rw [List.mem_flatMap] at c_mem
-              rcases c_mem with ⟨t, t_mem, c_mem⟩
-              rw [List.mem_map] at t_mem
-              rcases t_mem with ⟨v, v_mem, t_mem⟩
-              rcases FunctionFreeConjunction.mem_vars.mp (origin.fst.val.rule.frontier_subset_vars_body v_mem) with ⟨a, a_mem, v_mem'⟩
-              exists origin.fst.val.subs.apply_function_free_atom a
+            apply ih
+            rw [List.mem_flatMap] at c_mem
+            rcases c_mem with ⟨t, t_mem, c_mem⟩
+            rw [List.mem_map] at t_mem
+            rcases t_mem with ⟨v, v_mem, t_mem⟩
+            rcases FunctionFreeConjunction.mem_vars.mp (origin.fst.val.rule.frontier_subset_vars_body v_mem) with ⟨a, a_mem, v_mem'⟩
+            exists origin.fst.val.subs.apply_function_free_atom a
+            constructor
+            . have := cd2.active_trigger_origin_next next_eq
+              apply this.left
+              rw [List.mem_toSet]
+              unfold PreTrigger.mapped_body
+              unfold GroundSubstitution.apply_function_free_conj
+              apply List.mem_map_of_mem
+              exact a_mem
+            . unfold Fact.constants
+              rw [List.mem_flatMap]
+              exists t
               constructor
-              . have := cb.origin_trg_is_active i node eq
-                apply this.left
-                rw [List.mem_toSet]
-                unfold PreTrigger.mapped_body
-                unfold GroundSubstitution.apply_function_free_conj
-                apply List.mem_map_of_mem
-                exact a_mem
-              . unfold Fact.constants
-                rw [List.mem_flatMap]
-                exists t
+              . unfold GroundSubstitution.apply_function_free_atom
+                unfold TermMapping.apply_generalized_atom
+                rw [List.mem_map]
+                exists VarOrConst.var v
                 constructor
-                . unfold GroundSubstitution.apply_function_free_atom
-                  unfold TermMapping.apply_generalized_atom
-                  rw [List.mem_map]
-                  exists VarOrConst.var v
-                  constructor
-                  . exact v_mem'
-                  . unfold PreTrigger.subs_for_mapped_head at t_mem
-                    rw [PreTrigger.apply_to_var_or_const_frontier_var] at t_mem
-                    . exact t_mem
-                    . exact v_mem
-                . exact c_mem
+                . exact v_mem'
+                . unfold PreTrigger.subs_for_mapped_head at t_mem
+                  rw [PreTrigger.apply_to_var_or_const_frontier_var] at t_mem
+                  . exact t_mem
+                  . exact v_mem
+              . exact c_mem
           | inr c_mem =>
             apply Or.inr
             exists origin.fst.val.rule
@@ -215,271 +416,263 @@ namespace ChaseBranch
               . exact c_mem
         . exact c_mem
 
-  theorem trg_loaded_at_some_step_of_trg_loaded_for_result (cb : ChaseBranch obs kb) : ∀ trg : Trigger obs, trg.loaded cb.result -> ∃ n : Nat, (cb.branch.get? n).is_some_and (fun fs => trg.loaded fs.facts.val) := by
-    intro trg
-    unfold ChaseBranch.result
-    unfold PreTrigger.loaded
-
-    induction trg.mapped_body
-    case nil =>
-      intro _
-      exists 0
-      rw [← PossiblyInfiniteList.head_eq, cb.database_first]
-      simp [Option.is_some_and]
-      intro _ contra
-      simp [List.mem_toSet] at contra
-    case cons hd tl ih =>
-      intro loaded
-      rcases loaded hd (by simp [List.mem_toSet]) with ⟨hd_idx, hd_mem⟩
-      rw [Option.is_some_and_iff] at hd_mem
-
-      rcases ih (by intro e e_mem; rw [List.mem_toSet] at e_mem; apply loaded; simp [List.mem_toSet, e_mem]) with ⟨tl_idx, tl_mem⟩
-      rw [Option.is_some_and_iff] at tl_mem
-
-      exists max hd_idx tl_idx
-      rw [Option.is_some_and_iff]
-
-      cases Decidable.em (tl_idx ≤ hd_idx) with
-      | inl le =>
-        rcases hd_mem with ⟨node, node_eq, hd_mem⟩
-        exists node
+  theorem facts_mem_some_node_of_mem_result {cd : ChaseDerivation obs rules} : ∀ (l : List (Fact sig)), l.toSet ⊆ cd.result -> ∃ node ∈ cd, l.toSet ⊆ node.facts := by
+    intro l
+    induction l with
+    | nil => intros; exists cd.head; constructor; exact cd.head_mem; intro _ contra; simp [List.mem_toSet] at contra
+    | cons f l ih =>
+      intro subset
+      rcases subset f (by simp [List.mem_toSet]) with ⟨node_f, node_f_mem, f_mem⟩
+      rcases ih (by intro f f_mem; apply subset; rw [List.mem_toSet] at f_mem; simp [List.mem_toSet, f_mem]) with ⟨node_ih, node_ih_mem, l_subset⟩
+      rcases cd.subderivation_of_node_mem node_f_mem with ⟨cd_f, cd_f_head, cd_f_suffix⟩
+      cases mem_suffix_of_mem cd_f_suffix _ node_ih_mem with
+      | inl mem_suffix =>
+        exists node_f
         constructor
-        . rw [Nat.max_eq_left le]
-          exact node_eq
+        . exact node_f_mem
         . intro e e_mem
           rw [List.mem_toSet, List.mem_cons] at e_mem
           cases e_mem with
-          | inl e_mem => rw [e_mem]; exact hd_mem
-          | inr e_mem =>
-            rcases tl_mem with ⟨tl_node, tl_node_eq, tl_mem⟩
-            have := cb.stepIsSubsetOfAllFollowing tl_idx tl_node tl_node_eq (hd_idx - tl_idx)
-            rw [PossiblyInfiniteList.get?_drop, Nat.add_sub_cancel' le] at this
-            rw [node_eq, Option.is_none_or] at this
-            apply this
-            apply tl_mem
-            rw [List.mem_toSet]
-            exact e_mem
-      | inr le =>
-        have le := Nat.le_of_not_le le
-        rcases tl_mem with ⟨node, node_eq, tl_mem⟩
-        exists node
+          | inl e_mem => rw [e_mem]; exact f_mem
+          | inr e_mem => rw [← cd_f_head]; apply mem_suffix; apply l_subset; rw [List.mem_toSet]; exact e_mem
+      | inr mem_suffix =>
+        exists node_ih
         constructor
-        . rw [Nat.max_eq_right le]
-          exact node_eq
+        . exact node_ih_mem
         . intro e e_mem
           rw [List.mem_toSet, List.mem_cons] at e_mem
           cases e_mem with
-          | inr e_mem => apply tl_mem; rw [List.mem_toSet]; exact e_mem
+          | inr e_mem => apply l_subset; rw [List.mem_toSet]; exact e_mem
           | inl e_mem =>
-            rcases hd_mem with ⟨hd_node, hd_node_eq, hd_mem⟩
-            have := cb.stepIsSubsetOfAllFollowing hd_idx hd_node hd_node_eq (tl_idx - hd_idx)
-            rw [PossiblyInfiniteList.get?_drop, Nat.add_sub_cancel' le] at this
-            rw [node_eq, Option.is_none_or] at this
-            apply this
             rw [e_mem]
-            exact hd_mem
+            apply cd_f.facts_node_subset_every_mem _ mem_suffix
+            rw [cd_f_head]; exact f_mem
 
-  theorem trg_active_at_some_step_of_trg_active_for_result (cb : ChaseBranch obs kb) : ∀ trg : Trigger obs, trg.active cb.result -> ∃ n : Nat, (cb.branch.get? n).is_some_and (fun fs => trg.active fs.facts) := by
-    intro trg
-    intro active
-    rcases cb.trg_loaded_at_some_step_of_trg_loaded_for_result trg active.left with ⟨step, loaded_step⟩
-    rw [Option.is_some_and_iff] at loaded_step
-    rcases loaded_step with ⟨node, node_eq, loaded_step⟩
-    exists step
-    rw [Option.is_some_and_iff]
-    exists node
+  theorem trg_loaded_for_some_node_of_trg_loaded_for_result {cd : ChaseDerivation obs rules} : ∀ trg : Trigger obs, trg.loaded cd.result -> ∃ node ∈ cd, trg.loaded node.facts := by
+    intro trg trg_loaded
+    apply cd.facts_mem_some_node_of_mem_result
+    exact trg_loaded
+
+  theorem trg_active_for_some_node_of_trg_active_for_result {cd : ChaseDerivation obs rules} : ∀ trg : Trigger obs, trg.active cd.result -> ∃ node ∈ cd, trg.active node.facts := by
+    intro trg trg_active
+    rcases cd.trg_loaded_for_some_node_of_trg_loaded_for_result trg trg_active.left with ⟨node, node_mem, loaded_node⟩
+    exists node; simp only [node_mem, true_and]
+    constructor; exact loaded_node
+    intro contra
+    apply trg_active.right
+    exact obs.monotone (cd.facts_node_subset_result _ node_mem) contra
+
+  theorem result_models_rules {cd : ChaseDerivation obs rules} : cd.result.modelsRules rules := by
+    intro r r_mem subs subs_loaded
+    let trg : Trigger obs := ⟨r, subs⟩
+    have trg_loaded : trg.loaded cd.result := subs_loaded
+    apply obs.cond_implies_trg_is_satisfied (trg := trg)
+    rcases cd.trg_loaded_for_some_node_of_trg_loaded_for_result trg trg_loaded with ⟨node_loaded, node_loaded_mem, trg_loaded⟩
+    rcases cd.subderivation_of_node_mem node_loaded_mem with ⟨cd_loaded, cd_loaded_head, cd_loaded_suffix⟩
+    rcases cd_loaded.fairness' ⟨trg, r_mem⟩ with ⟨cd_obs, cd_obs_suffix, fairness⟩
+    specialize fairness cd_obs.head cd_obs.head_mem
+    apply Classical.byContradiction
+    intro contra_not_obs
+    apply fairness
     constructor
-    . exact node_eq
-    . constructor
-      . exact loaded_step
-      . intro contra
-        apply active.right
-        apply obs.monotone
-        . have := cb.stepIsSubsetOfResult step
-          rw [node_eq, Option.is_none_or] at this
-          exact this
-        . exact contra
-
-  theorem result_models_kb (cb : ChaseBranch obs kb) : cb.result.modelsKb kb := by
-    constructor
-    . unfold FactSet.modelsDb
-      unfold ChaseBranch.result
-      intro f h
-      exists 0
-      rw [← PossiblyInfiniteList.head_eq, cb.database_first, Option.is_some_and]
-      exact h
-    . unfold FactSet.modelsRules
-      intro r h
-      unfold FactSet.modelsRule
-      intro subs subs_loaded
-      apply Classical.byContradiction
-      intro subs_not_obsolete
-      let trg : Trigger obs := ⟨r, subs⟩
-      have trg_loaded : trg.loaded cb.result := by apply subs_loaded
-      have trg_not_obsolete : ¬ obs.cond trg cb.result := by
-        intro contra
-        have obs_impl_sat := obs.cond_implies_trg_is_satisfied contra
-        apply subs_not_obsolete
-        rcases obs_impl_sat with ⟨i, s', obs_impl_sat⟩
-        exists i
-        exists s'
-
-      rcases cb.trg_active_at_some_step_of_trg_active_for_result trg ⟨trg_loaded, trg_not_obsolete⟩ with ⟨step, step_active⟩
-      rw [Option.is_some_and_iff] at step_active
-      rcases step_active with ⟨node, node_eq, step_active⟩
-
-      rcases cb.fairness ⟨trg, by apply h⟩ with ⟨step', step'_not_active⟩
-      rw [Option.is_some_and_iff] at step'_not_active
-      rcases step'_not_active.left with ⟨node', node'_eq, step'_not_active_left⟩
-
-      apply step'_not_active_left
-      constructor
-      . cases Decidable.em (step ≤ step') with
-        | inl le =>
-          apply Set.subset_trans (b := node.facts.val)
-          . exact step_active.left
-          . have := cb.stepIsSubsetOfAllFollowing step node node_eq (step' - step)
-            rw [PossiblyInfiniteList.head_eq, PossiblyInfiniteList.get?_drop, Nat.add_zero] at node'_eq
-            rw [PossiblyInfiniteList.get?_drop, Nat.add_sub_cancel' le, node'_eq, Option.is_none_or] at this
-            exact this
-        | inr le =>
-          have gt := Nat.gt_of_not_le le
-          apply False.elim
-          rcases Nat.exists_eq_add_of_lt gt with ⟨j, gt⟩
-          have := step'_not_active.right j
-          rw [Nat.add_one, ← Nat.add_succ] at gt
-          rw [PossiblyInfiniteList.get?_tail, PossiblyInfiniteList.get?_drop, ← gt] at this
-          rw [node_eq, Option.is_none_or] at this
-          apply this
-          exact step_active
-      . intro contra
-        apply trg_not_obsolete
-        apply obs.monotone
-        . have := cb.stepIsSubsetOfResult step'
-          rw [PossiblyInfiniteList.head_eq, PossiblyInfiniteList.get?_drop, Nat.add_zero] at node'_eq
-          rw [node'_eq, Option.is_none_or] at this
-          exact this
-        . exact contra
+    . apply Set.subset_trans trg_loaded
+      rw [← cd_loaded_head]
+      apply cd_loaded.facts_node_subset_every_mem
+      apply cd_obs.mem_of_mem_suffix cd_obs_suffix
+      apply cd_obs.head_mem
+    . intro contra
+      apply contra_not_obs
+      rw [← result_suffix (PossiblyInfiniteList.IsSuffix_trans cd_obs_suffix cd_loaded_suffix)]
+      apply obs.monotone
+      . apply cd_obs.facts_node_subset_result; apply cd_obs.head_mem
+      . exact contra
 
   theorem functional_term_originates_from_some_trigger
-      {cb : ChaseBranch obs kb} {step : Nat} {node : ChaseNode obs kb.rules}
-      (eq : (cb.branch.drop step).head = some node)
+      {cd : ChaseDerivation obs rules}
+      (node : Node cd)
       {t : GroundTerm sig}
       (t_is_func : ∃ func ts arity_ok, t = GroundTerm.func func ts arity_ok)
-      (t_mem : t ∈ node.facts.val.terms) :
-      ∃ step2, step2 ≤ step ∧ (cb.branch.drop step2).head.is_some_and (fun node2 => node2.origin.is_some_and (fun origin => t ∈ origin.fst.val.fresh_terms_for_head_disjunct origin.snd.val (by rw [← PreTrigger.length_mapped_head]; exact origin.snd.isLt))) := by
-    induction step generalizing node with
-    | zero =>
-      rw [PossiblyInfiniteList.drop_zero, cb.database_first] at eq
-      rw [Option.some.injEq] at eq
-      have func_free := kb.db.toFactSet.property.right
-      unfold FactSet.isFunctionFree at func_free
-      rcases t_mem with ⟨f, f_mem, t_mem⟩
-      rw [← eq] at f_mem
-      specialize func_free f f_mem
-      unfold Fact.isFunctionFree at func_free
-      specialize func_free _ t_mem
-      rcases func_free with ⟨_, func_free⟩
-      rcases t_is_func with ⟨_, _, _, t_is_func⟩
-      rw [t_is_func] at func_free
-      simp [GroundTerm.func, GroundTerm.const] at func_free
-    | succ step ih =>
-      let prev_node := (cb.prev_node step (by rw [PossiblyInfiniteList.head_eq, PossiblyInfiniteList.get?_drop] at eq; simp [PossiblyInfiniteList.head_eq, PossiblyInfiniteList.get?_tail, PossiblyInfiniteList.get?_drop, eq]))
-      cases Classical.em (t ∈ prev_node.facts.val.terms) with
-      | inl term_in_prev_node =>
-        rcases ih (by apply cb.prev_node_eq) term_in_prev_node with ⟨step2, ih⟩
-        exists step2, (Nat.le_succ_of_le ih.left)
-        exact ih.right
-      | inr term_not_in_prev_node =>
-        exists (step+1), (by simp)
-        rw [Option.is_some_and_iff]
-        exists node
-        constructor
-        . exact eq
-        rw [Option.is_some_and_iff]
-        let origin := node.origin.get (cb.origin_isSome step eq)
-        exists origin
-        constructor
-        . simp [origin]
-        rcases t_mem with ⟨f, f_mem, t_mem⟩
-        rw [cb.origin_trg_result_yields_next_node_facts _ _ eq] at f_mem
-        cases f_mem with
-        | inl f_mem => apply False.elim; apply term_not_in_prev_node; exists f
-        | inr f_mem =>
-          have t_mem : t ∈ origin.fst.val.mapped_head[origin.snd.val].flatMap GeneralizedAtom.terms := by
-            rw [List.mem_flatMap]; exists f
-          rw [PreTrigger.mem_terms_mapped_head_iff] at t_mem
-          cases t_mem with
-          | inl t_mem =>
-            rcases t_is_func with ⟨_, _, _, t_is_func⟩
-            rcases t_mem with ⟨_, _, t_mem⟩
-            rw [t_is_func] at t_mem
-            simp [GroundTerm.const, GroundTerm.func] at t_mem
-          | inr t_mem =>
-          cases t_mem with
-          | inl t_mem =>
-            apply False.elim; apply term_not_in_prev_node
-            apply FactSet.terms_subset_of_subset (cb.origin_trg_is_active step node eq).left
-            rw [FactSet.mem_terms_toSet]
-            rw [PreTrigger.mem_terms_mapped_body_iff]
-            apply Or.inr
-            rw [List.mem_map] at t_mem; rcases t_mem with ⟨v, v_mem, t_mem⟩
-            exists v
-            constructor
-            . apply Rule.frontier_subset_vars_body; apply Rule.mem_frontier_iff_mem_frontier_for_head.mpr; exact ⟨_, v_mem⟩
-            . exact t_mem
-          | inr t_mem => exact t_mem
+      (t_mem : t ∈ node.val.facts.terms) :
+      t ∈ cd.head.facts.terms ∨ ∃ node2, node2 ≼ node ∧ node2.val.origin.is_some_and (fun origin => t ∈ origin.fst.val.fresh_terms_for_head_disjunct origin.snd.val (by rw [← PreTrigger.length_mapped_head]; exact origin.snd.isLt)) := by
+    induction node using mem_rec with
+    | head => apply Or.inl; exact t_mem
+    | step cd2 suffix ih next next_mem =>
+      rw [cd2.facts_next next_mem, FactSet.terms_union] at t_mem
+
+      have aux : t ∈ cd2.head.facts.terms -> t ∈ cd.head.facts.terms ∨ ∃ (node2 : cd.Node), node2 ≼ ⟨next, cd2.mem_of_mem_suffix suffix _ (cd2.next_mem_of_mem _ next_mem)⟩ ∧ node2.val.origin.is_some_and (fun origin => t ∈ origin.fst.val.fresh_terms_for_head_disjunct origin.snd.val (by rw [← PreTrigger.length_mapped_head]; exact origin.snd.isLt)) := by
+        intro t_mem
+        cases ih t_mem with
+        | inl ih => apply Or.inl; exact ih
+        | inr ih =>
+          rcases ih with ⟨node2, prec, t_mem⟩
+          apply Or.inr; exists node2; constructor;
+          . apply predecessor_trans prec
+            exact predecessor_of_suffix suffix (head_prec_next next_mem)
+          . exact t_mem
+
+      cases t_mem with
+      | inl t_mem => exact aux t_mem
+      | inr t_mem =>
+        unfold ChaseNode.origin_result at t_mem
+        rw [FactSet.mem_terms_toSet, PreTrigger.mem_terms_mapped_head_iff] at t_mem
+        cases t_mem with
+        | inl t_mem => rcases t_is_func with ⟨func, ts, arity, t_is_func⟩; rcases t_mem with ⟨c, _, t_mem⟩; rw [← t_mem] at t_is_func; simp [GroundTerm.const, GroundTerm.func] at t_is_func
+        | inr t_mem =>
+        cases t_mem with
+        | inr t_mem =>
+          apply Or.inr; exists ⟨next, cd2.mem_of_mem_suffix suffix _ (cd2.next_mem_of_mem _ next_mem)⟩; constructor
+          . exact predecessor_refl
+          . rw [Option.is_some_and_iff]
+            exists next.origin.get (cd2.isSome_origin_next next_mem)
+            simp only [Option.some_get, true_and]
+            exact t_mem
+        | inl t_mem =>
+          apply aux
+          apply FactSet.terms_subset_of_subset (cd2.active_trigger_origin_next next_mem).left
+          rw [List.mem_map] at t_mem
+          rcases t_mem with ⟨v, v_mem, t_mem⟩
+          rw [FactSet.mem_terms_toSet, PreTrigger.mem_terms_mapped_body_iff]
+          apply Or.inr
+          exists v; simp only [t_mem, and_true]
+          apply Rule.frontier_subset_vars_body; rw [Rule.mem_frontier_iff_mem_frontier_for_head]; exact ⟨_, v_mem⟩
 
   theorem trigger_introducing_functional_term_occurs_in_chase
-      {cb : ChaseBranch obs kb} {step : Nat} {node : ChaseNode obs kb.rules}
-      (eq : (cb.branch.drop step).head = some node)
+      {cd : ChaseDerivation obs rules}
+      (node : Node cd)
       {t : GroundTerm sig}
-      (t_mem_node : t ∈ node.facts.val.terms)
-      {trg : RTrigger obs kb.rules}
+      (t_mem_node : t ∈ node.val.facts.terms)
+      {trg : RTrigger obs rules}
       {disj_idx : Nat}
       {lt : disj_idx < trg.val.rule.head.length}
       (t_mem_trg : t ∈ trg.val.fresh_terms_for_head_disjunct disj_idx lt) :
-      ∃ step2, step2 ≤ step ∧ (cb.branch.drop step2).head.is_some_and (fun node2 => node2.origin.is_some_and (fun origin => origin.fst.equiv trg ∧ origin.snd.val = disj_idx)) := by
-    rcases functional_term_originates_from_some_trigger eq (by
+      t ∈ cd.head.facts.terms ∨ ∃ node2, node2 ≼ node ∧ node2.val.origin.is_some_and (fun origin => origin.fst.equiv trg ∧ origin.snd.val = disj_idx) := by
+    cases functional_term_originates_from_some_trigger node (by
       cases eq : t with
       | const _ =>
         rw [eq] at t_mem_trg
         simp [PreTrigger.fresh_terms_for_head_disjunct, PreTrigger.functional_term_for_var, GroundTerm.func, GroundTerm.const] at t_mem_trg
       | func func ts arity_ok => exists func, ts, arity_ok
-    ) t_mem_node with ⟨step2, le, h⟩
-    simp only [Option.is_some_and_iff] at h
-    rcases h with ⟨node2, node2_eq, origin, origin_eq, t_mem_origin⟩
-    simp only [Option.is_some_and_iff]
-    exists step2; constructor
-    . exact le
-    exists node2; constructor
-    . exact node2_eq
-    exists origin; constructor
-    . exact origin_eq
-    exact RTrigger.equiv_of_term_mem_fresh_terms_for_head_disjunct t_mem_origin t_mem_trg
+    ) t_mem_node with
+    | inl t_mem => apply Or.inl; exact t_mem
+    | inr t_mem =>
+      apply Or.inr
+      simp only [Option.is_some_and_iff] at t_mem
+      rcases t_mem with ⟨node2, prec, origin, origin_eq, t_mem⟩
+      simp only [Option.is_some_and_iff]
+      exists node2; simp only [prec, true_and]
+      exists origin; simp only [origin_eq, true_and]
+      exact RTrigger.equiv_of_term_mem_fresh_terms_for_head_disjunct t_mem t_mem_trg
 
   theorem result_of_trigger_introducing_functional_term_occurs_in_chase
-      {cb : ChaseBranch obs kb} {step : Nat} {node : ChaseNode obs kb.rules}
-      (eq : (cb.branch.drop step).head = some node)
+      {cd : ChaseDerivation obs rules}
+      (node : Node cd)
       {t : GroundTerm sig}
-      (t_mem_node : t ∈ node.facts.val.terms)
+      (t_mem_node : t ∈ node.val.facts.terms)
+      {trg : RTrigger obs rules}
+      {disj_idx : Nat}
+      {lt : disj_idx < trg.val.rule.head.length}
+      (t_mem_trg : t ∈ trg.val.fresh_terms_for_head_disjunct disj_idx lt) :
+      t ∈ cd.head.facts.terms ∨ (trg.val.mapped_head[disj_idx]'(by rw [PreTrigger.length_mapped_head]; exact lt)).toSet ⊆ node.val.facts := by
+    cases trigger_introducing_functional_term_occurs_in_chase node t_mem_node t_mem_trg with
+    | inl t_mem => apply Or.inl; exact t_mem
+    | inr t_mem =>
+      apply Or.inr
+      simp only [Option.is_some_and_iff] at t_mem
+      rcases t_mem with ⟨node2, prec, origin, origin_eq, equiv, index_eq⟩
+      apply Set.subset_trans _ (cd.facts_node_subset_of_prec prec)
+      have := node2.val.facts_contain_origin_result
+      simp only [origin_eq, Option.is_none_or] at this
+      simp only [← PreTrigger.result_eq_of_equiv equiv, ← index_eq]
+      exact this
+
+end ChaseDerivation
+
+structure ChaseBranch (obs : ObsoletenessCondition sig) (kb : KnowledgeBase sig) extends ChaseDerivation obs kb.rules where
+  database_first : branch.head = some {
+    facts := kb.db.toFactSet,
+    origin := none,
+    facts_contain_origin_result := by simp [Option.is_none_or]
+  }
+
+namespace ChaseBranch
+
+  variable {obs : ObsoletenessCondition sig} {kb : KnowledgeBase sig}
+
+  theorem database_first' {cb : ChaseBranch obs kb} : cb.head = {
+    facts := kb.db.toFactSet,
+    origin := none,
+    facts_contain_origin_result := by simp [Option.is_none_or]
+  } := by simp only [ChaseDerivation.head, cb.database_first, Option.get_some]
+
+  theorem facts_finite_of_mem {cb : ChaseBranch obs kb} (node : cb.Node) : node.val.facts.finite := by
+    induction node using ChaseDerivation.mem_rec with
+    | head => simp only [database_first']; exact kb.db.toFactSet.property.left
+    | step cd2 suffix ih next next_mem =>
+      rw [cd2.facts_next next_mem]
+      apply Set.union_finite_of_both_finite ih
+      apply List.finite_toSet
+
+  theorem func_term_not_mem_head {cb : ChaseBranch obs kb} {t : GroundTerm sig} (t_is_func : ∃ func ts arity_ok, t = GroundTerm.func func ts arity_ok) : ¬ t ∈ cb.head.facts.terms := by
+    intro t_mem
+    simp only [database_first'] at t_mem
+    rcases t_mem with ⟨f, f_mem, t_mem⟩
+    rcases kb.db.toFactSet.property.right f f_mem t t_mem with ⟨c, t_eq⟩
+    rcases t_is_func with ⟨_, _, _, t_eq'⟩
+    rw [t_eq'] at t_eq
+    simp [GroundTerm.const, GroundTerm.func] at t_eq
+
+  theorem constants_node_subset_constants_db_union_constants_rules {cb : ChaseBranch obs kb} {node : cb.Node} :
+      node.val.facts.constants ⊆ (kb.db.constants.val ∪ kb.rules.head_constants) := by
+    have := cb.constants_node_subset_constants_fs_union_constants_rules node.property
+    simp only [cb.database_first', Database.toFactSet_constants_same] at this
+    exact this
+
+  theorem result_models_kb {cb : ChaseBranch obs kb} : cb.result.modelsKb kb := by
+    constructor
+    . intro f h
+      apply cb.facts_node_subset_result cb.head
+      . apply cb.head_mem
+      . rw [database_first']; exact h
+    . exact cb.result_models_rules
+
+  theorem functional_term_originates_from_some_trigger
+      {cb : ChaseBranch obs kb}
+      (node : cb.Node)
+      {t : GroundTerm sig}
+      (t_is_func : ∃ func ts arity_ok, t = GroundTerm.func func ts arity_ok)
+      (t_mem : t ∈ node.val.facts.terms) :
+      ∃ node2, node2 ≼ node ∧ node2.val.origin.is_some_and (fun origin => t ∈ origin.fst.val.fresh_terms_for_head_disjunct origin.snd.val (by rw [← PreTrigger.length_mapped_head]; exact origin.snd.isLt)) := by
+    cases ChaseDerivation.functional_term_originates_from_some_trigger node t_is_func t_mem with
+    | inl t_mem => apply False.elim; exact cb.func_term_not_mem_head t_is_func t_mem
+    | inr t_mem => exact t_mem
+
+  theorem trigger_introducing_functional_term_occurs_in_chase
+      {cb : ChaseBranch obs kb}
+      (node : cb.Node)
+      {t : GroundTerm sig}
+      (t_mem_node : t ∈ node.val.facts.terms)
       {trg : RTrigger obs kb.rules}
       {disj_idx : Nat}
       {lt : disj_idx < trg.val.rule.head.length}
       (t_mem_trg : t ∈ trg.val.fresh_terms_for_head_disjunct disj_idx lt) :
-      (trg.val.mapped_head[disj_idx]'(by rw [PreTrigger.length_mapped_head]; exact lt)).toSet ⊆ node.facts.val := by
-    rcases trigger_introducing_functional_term_occurs_in_chase eq t_mem_node t_mem_trg with ⟨step2, le, h⟩
-    simp only [Option.is_some_and_iff] at h
-    rcases h with ⟨node2, node2_eq, origin, origin_eq, equiv, index_eq⟩
-    have subset_following := cb.stepIsSubsetOfAllFollowing step2 node2 node2_eq (step - step2)
-    rw [PossiblyInfiniteList.get?_drop, Nat.add_sub_of_le le] at subset_following
-    rw [PossiblyInfiniteList.head_drop] at eq
-    simp only [eq, Option.is_none_or] at subset_following
-    apply Set.subset_trans _ subset_following
-    have := node2.facts_contain_origin_result
-    simp only [origin_eq, Option.is_none_or] at this
-    simp only [← PreTrigger.result_eq_of_equiv equiv, ← index_eq]
-    exact this
+      ∃ node2, node2 ≼ node ∧ node2.val.origin.is_some_and (fun origin => origin.fst.equiv trg ∧ origin.snd.val = disj_idx) := by
+    cases ChaseDerivation.trigger_introducing_functional_term_occurs_in_chase node t_mem_node t_mem_trg with
+    | inl t_mem => apply False.elim; exact cb.func_term_not_mem_head (PreTrigger.term_functional_of_mem_fresh_terms _ t_mem_trg) t_mem
+    | inr t_mem => exact t_mem
+
+  theorem result_of_trigger_introducing_functional_term_occurs_in_chase
+      {cb : ChaseBranch obs kb}
+      (node : cb.Node)
+      {t : GroundTerm sig}
+      (t_mem_node : t ∈ node.val.facts.terms)
+      {trg : RTrigger obs kb.rules}
+      {disj_idx : Nat}
+      {lt : disj_idx < trg.val.rule.head.length}
+      (t_mem_trg : t ∈ trg.val.fresh_terms_for_head_disjunct disj_idx lt) :
+      (trg.val.mapped_head[disj_idx]'(by rw [PreTrigger.length_mapped_head]; exact lt)).toSet ⊆ node.val.facts := by
+    cases ChaseDerivation.result_of_trigger_introducing_functional_term_occurs_in_chase node t_mem_node t_mem_trg with
+    | inl t_mem => apply False.elim; exact cb.func_term_not_mem_head (PreTrigger.term_functional_of_mem_fresh_terms _ t_mem_trg) t_mem
+    | inr t_mem => exact t_mem
 
 end ChaseBranch
 
