ExistentialRules/AtomsAndFacts/Basic.lean
@@ -372,6 +372,14 @@ namespace FactSet
   theorem terms_subset_of_subset {fs1 fs2 : FactSet sig} : fs1 ⊆ fs2 -> fs1.terms ⊆ fs2.terms := by
     rintro sub t ⟨f, f_mem, t_mem⟩; exists f; exact ⟨sub _ f_mem, t_mem⟩
 
+  theorem terms_union {fs1 fs2 : FactSet sig} : (fs1 ∪ fs2).terms = fs1.terms ∪ fs2.terms := by
+    apply Set.ext
+    intro t; constructor
+    . rintro ⟨f, f_mem, t_mem⟩; cases f_mem with | inl f_mem => apply Or.inl; exists f | inr f_mem => apply Or.inr; exists f
+    . intro t_mem; cases t_mem with
+      | inl t_mem => rcases t_mem with ⟨f, f_mem, t_mem⟩; exists f; simp only [t_mem, and_true]; exact Or.inl f_mem
+      | inr t_mem => rcases t_mem with ⟨f, f_mem, t_mem⟩; exists f; simp only [t_mem, and_true]; exact Or.inr f_mem
+
   theorem terms_finite_of_finite (fs : FactSet sig) (finite : fs.finite) : fs.terms.finite := by
     rcases finite with ⟨l, nodup, finite⟩
     exists (l.map GeneralizedAtom.terms).flatten.eraseDupsKeepRight
@@ -403,6 +411,15 @@ namespace FactSet
   theorem mem_constants_toSet {l : List (Fact sig)} : ∀ c, c ∈ FactSet.constants (l.toSet) ↔ c ∈ l.flatMap Fact.constants := by
     intro t; rw [List.mem_flatMap]
     constructor <;> (rintro ⟨f, f_mem, t_mem⟩; exists f)
+
+  theorem constants_union {fs1 fs2 : FactSet sig} : (fs1 ∪ fs2).constants = fs1.constants ∪ fs2.constants := by
+    -- NOTE: same proof as terms_union
+    apply Set.ext
+    intro t; constructor
+    . rintro ⟨f, f_mem, t_mem⟩; cases f_mem with | inl f_mem => apply Or.inl; exists f | inr f_mem => apply Or.inr; exists f
+    . intro t_mem; cases t_mem with
+      | inl t_mem => rcases t_mem with ⟨f, f_mem, t_mem⟩; exists f; simp only [t_mem, and_true]; exact Or.inl f_mem
+      | inr t_mem => rcases t_mem with ⟨f, f_mem, t_mem⟩; exists f; simp only [t_mem, and_true]; exact Or.inr f_mem
 
   theorem constants_finite_of_finite (fs : FactSet sig) (fin : fs.finite) : fs.constants.finite := by
     rcases fin with ⟨l, _, l_eq⟩
